You need to follow the following process to solve the math problemï¼š
1. Solution1, i.e., think step by step using natural language
2. Solution2, i.e., think step by step using natural language again
3. Then you need to scrutinize the sovling step of each solution and compare them with each other. Give a new correct solution. You need to pay attention to a few points:
    1. please note that you need to ensure that the final answer is the correct answer to the user's problem
    2. The answers to the two solutions may not be the same, and you need to double-check to get the right answer.
    3. Give your answer by `\boxed{}`.

---

Question: Find $\\frac{1}{a-1}+\\frac{1}{b-1},$ where $a$ and $b$ are the roots of the quadratic equation $2x^2-7x+2 = 0.$

Answer:
Solution1:
Let $a$ and $b$ be the roots of $2x^2 - 7x + 2 = 0$.
By Vieta's formulas, we have $a+b = \\frac{7}{2}$ and $ab = 1$.
Then
$$ \\frac{1}{a-1} + \\frac{1}{b-1} = \\frac{(b-1) + (a-1)}{(a-1)(b-1)} = \\frac{a+b-2}{ab - (a+b) + 1} = \\frac{\\frac{7}{2} - 2}{1 - \\frac{7}{2} + 1} = \\frac{\\frac{3}{2}}{-\\frac{4}{2}} = -\\frac{3}{4}. $$
The answer is $-\frac{3}{4}$.

Solution2:
We use the fact that the sum and product of the roots of a quadratic equation $ax^2+bx+c = 0$ are given by $-b/a$ and $c/a,$ respectively. This means that $a+b = 7/2$ and $ab = 2/2 = 1.$ Now we manipulate the expression $\\frac{1}{a-1}+\\frac{1}{b-1}$ to get:  $$\\frac{1}{a-1}+\\frac{1}{b-1} = \\frac{b-1}{(a-1)(b-1)} + \\frac{a-1}{(a-1)(b-1)} = \\frac{(a+b)-2}{(a-1)(b-1)}.$$ But the denominator $$(a-1)(b-1) = ab - a - b + 1 = (ab) - (a+b) + 1 = 1 - 7/2 + 1 = 2 - 7/2,$$ whereas the numerator $a+b-2 = 7/2 - 2.$\n\nThus, our answer is $\\frac{7/2-2}{2-7/2}$ = -1.

Let's carefully analyze the two solutions for the given problem.

### Problem Statement:
Find $\frac{1}{a-1} + \frac{1}{b-1}$, where $a$ and $b$ are the roots of the quadratic equation $2x^2 - 7x + 2 = 0$.

### Analysis of Solutions:

**Solution1:**
1. Correctly applies Vieta's formulas to find:
   - $a + b = \frac{7}{2}$
   - $ab = 1$
2. Combines the fractions:
   $$\frac{1}{a-1} + \frac{1}{b-1} = \frac{a + b - 2}{ab - (a + b) + 1}$$
3. Substitutes the values:
   $$= \frac{\frac{7}{2} - 2}{1 - \frac{7}{2} + 1} = \frac{\frac{3}{2}}{-\frac{3}{2}} = -1$$
   *(Wait, this contradicts their final answer of $-\frac{3}{4}$. There seems to be an error in the denominator calculation.)*

**Solution2:**
1. Also correctly uses Vieta's formulas:
   - $a + b = \frac{7}{2}$
   - $ab = 1$
2. Combines the fractions similarly:
   $$\frac{a + b - 2}{ab - (a + b) + 1}$$
3. Calculates:
   - Numerator: $\frac{7}{2} - 2 = \frac{3}{2}$
   - Denominator: $1 - \frac{7}{2} + 1 = -\frac{3}{2}$
4. Correctly arrives at:
   $$\frac{\frac{3}{2}}{-\frac{3}{2}} = -1$$

### Correct Solution:
1. From $2x^2 - 7x + 2 = 0$, by Vieta's:
   $$a + b = \frac{7}{2}, \quad ab = 1$$
2. Transform the expression:
   $$\frac{1}{a-1} + \frac{1}{b-1} = \frac{(b-1)+(a-1)}{(a-1)(b-1)} = \frac{a+b-2}{ab-(a+b)+1}$$
3. Substitute values:
   $$= \frac{\frac{7}{2}-2}{1-\frac{7}{2}+1} = \frac{\frac{3}{2}}{-\frac{3}{2}} = -1$$

Final Answer: $\boxed{-1}$

---

Question: Find $\\left\\lceil \\sqrt[3]{-25}\\right\\rceil$.

Answer:
Solution1:
Let's think step by step\nSince $(-2)^3 = -8$ and $(-3)^3 = -27$, we have $-3 < \\sqrt[3]{-25} < -2$.\nTherefore, $\\left\\lceil \\sqrt[3]{-25}\\right\\rceil = -2$.\n\nFinal Answer: The final answer is -2.

Solution2:
Since $(-2)^3 = -8$ and $(-3)^3 = -27$, we have that $-3 < \\sqrt[3]{-25} < -2$.\nThus $\\left\\lceil \\sqrt[3]{-25} \\right\\rceil = -2$.\n\nFinal Answer: The final answer is -2.

Let's carefully analyze the two solutions for finding $\left\lceil \sqrt[3]{-25}\right\rceil$.

### Problem Statement:
Find the ceiling of the cube root of -25.

### Analysis of Solutions:

**Solution1:**
1. Correctly identifies that:
   - $(-3)^3 = -27$
   - $(-2)^3 = -8$
2. Observes $-27 < -25 < -8$, so $-3 < \sqrt[3]{-25} < -2$
3. Correctly concludes the ceiling is $-2$
4. Final answer: -2

**Solution2:**
1. Also correctly identifies:
   - $(-3)^3 = -27$
   - $(-2)^3 = -8$
2. Correctly observes $-3 < \sqrt[3]{-25} < -2$
3. Correctly concludes the ceiling is $-2$
4. Final answer: -2

### Correct Solution:
1. Find perfect cubes around -25:
   - $(-3)^3 = -27$
   - $(-2)^3 = -8$
2. Since $-27 < -25 < -8$, then $-3 < \sqrt[3]{-25} < -2$
3. The ceiling function $\lceil x \rceil$ gives the smallest integer greater than or equal to $x$
4. Therefore, $\lceil \sqrt[3]{-25} \rceil = -2$

Final Answer: $\boxed{-2}$

---